src/util.lean
@@ -1,0 +1,20 @@
+-- (C) Copyright 2019, Hans-Dieter Hiep
+
+universe u
+variable {α : Type u}
+
+inductive list_at: α → list α → Type u
+| head (x : α) (xs : list α): list_at x (x :: xs)
+| tail (x y : α) (l : list α): list_at x l → list_at x (y :: l)
+
+lemma list_at_mem {x : α} {l : list α} : list_at x l → x ∈ l :=
+begin
+    intro H,
+    induction l,
+    cases H,
+    cases H,
+    constructor, refl,
+    have: x ∈ l_tl,
+        apply l_ih, assumption,
+    right, assumption
+end
